\documentclass{article}
\usepackage{graphicx}
\usepackage{amsmath}
\usepackage{amsfonts}
\usepackage[margin=1.5cm]{geometry}  
\begin{document}

\textbf{\underline{Magnitude of Real-valued Polynomial over Complex Plane}}

\begin{align*}
    f_{N}(x)&= \sum^{N - 1}_{n = 0}c_{n}x^{n} \quad , \quad x \in \mathbb{C} \quad , \quad c_n \in \mathbb{R}, \quad , \quad n = 0, ..., N - 1 \\ \\
            &= \sum^{N - 1}_{n = 0}c_{n}|x|^{n}e^{jn\angle{x}} \\ \\
            &= \Big(\vec{c} \odot \vec{|x|}\Big)^{T}\vec{e^{j\angle{x}}} \quad , \quad
                                     \vec{c} \equiv \begin{bmatrix}
                                                        c_{N - 1} \\
                                                        c_{N - 2} \\
                                                        c_{N - 3} \\
                                                        \vdots \\
                                                        c_{2} \\
                                                        c_{1} \\
                                                        c_{0}
                                                      \end{bmatrix} \quad , \quad
                                   \vec{|x|} \equiv \begin{bmatrix}
                                                        |x|^{N - 1} \\
                                                        |x|^{N - 2} \\
                                                        |x|^{N - 3} \\
                                                        \vdots \\
                                                        |x|^{2} \\
                                                        |x| \\
                                                        1
                                                      \end{bmatrix} \quad , \quad
                \vec{e^{j\angle{x}}} \equiv \begin{bmatrix}
                                                e^{j(N - 1)\angle{x}^{\circ}} \\
                                                e^{j(N - 2)\angle{x}^{\circ}} \\
                                                e^{j(N - 3)\angle{x}^{\circ}} \\
                                                \vdots \\
                                                e^{j2\angle{x}^{\circ}} \\
                                                e^{j\angle{x}^{\circ}} \\
                                                1
                                              \end{bmatrix} \quad , \quad \\ \\
            &= \vec{m}^{T}\vec{e^{j\angle{x}}} \quad , \quad \vec{m} \equiv \vec{c} \odot \vec{|x|} 
\end{align*}

\begin{align*}
    \Big|f_{N}(x)\Big|^{2}&= f_{N}(x)f^{*}_{N}(x) \\ \\
                          &= \vec{m}^{T}\vec{e^{j\angle{x}}}\vec{e^{-j\angle{x}}}^{T}\vec{m} \\ \\
                          &= \vec{m}^{T}\Bigg(I_{N} + \sum_{n=1}^{N - 1}\Big(e^{nj\angle{x}}U_{N, n} + e^{-nj\angle{x}}U_{N, n}^{T}\Big)\Bigg)\vec{m} \quad , \quad U_{N, n} \equiv \begin{bmatrix}
                                                                                                                                                                                        0_{N - n, n} & I_{N - n} \\ \\
                                                                                                                                                                                        0_{n} & 0_{n, N - n}
                                                                                                                                                                                      \end{bmatrix} \\ \\
                          &= \vec{m}^{T}I_{N}\vec{m} + \sum_{n=1}^{N - 1}\Bigg(e^{nj\angle{x}}\vec{m}^{T}U_{N, n}\vec{m} + e^{-nj\angle{x}}\vec{m}^{T}U_{N, n}^{T}\vec{m}\Bigg) \\ \\
                          &= \vec{m}^{T}\vec{m} + \sum_{n=1}^{N - 1}\Bigg(e^{nj\angle{x}}\vec{m}^{T}U_{N, n}\vec{m} + e^{-nj\angle{x}}\vec{m}^{T}U_{N, n}\vec{m}\Bigg) \\ \\
                          &= \big|\vec{m}\big|^{2} + \sum_{n=1}^{N - 1}\Big(e^{nj\angle{x}} + e^{-nj\angle{x}}\Big)\Big(\vec{m}^{T}U_{N, n}\vec{m}\Big) \\ \\
                          &= \big|\vec{m}\big|^{2} + \sum_{n=1}^{N - 1}2\cos\big(n\angle{x}\big)M_{N, n} \quad , \quad M_{N, n} = \vec{m}^{T}U_{N, n}\vec{m} \\ \\
                          &= \big|\vec{m}\big|^{2} + 2\sum_{n=1}^{N - 1}M_{N, n}T_{n}\Big(\cos\big(\angle{x}\big)\Big)
\end{align*}

\textbf{\underline{Application towards Frequency Analysis}}

\begin{align*}
    & \Rightarrow x = z^{-1} \quad \quad \quad \quad \quad \quad \quad \quad \text{Z-transform, (Transformation of Complex Plane for Discrete-time analysis)} \\ \\
    & \Rightarrow x = \big(e^{j\omega}\big)^{-1} = e^{-j\omega} \quad \quad \quad \text{Discrete-Time Fourier Transform (Staying along unit circle)} \\ \\
    & \Rightarrow |x| = 1, \quad \angle{x} = \omega \\ \\
    & \Rightarrow \vec{|x|} = \begin{bmatrix}
                                    |x|^{N - 1} \\
                                    |x|^{N - 2} \\
                                    |x|^{N - 3} \\
                                    \vdots \\
                                    |x|^{2} \\
                                    |x| \\
                                    1
                                \end{bmatrix}
                            = \begin{bmatrix}
                                    1 \\
                                    1 \\
                                    1 \\
                                    \vdots
                                    1 \\
                                    1 \\
                                    1
                                \end{bmatrix} = \vec{1} \\ \\
    & \Rightarrow \vec{m} = \vec{c} \odot \vec{|x|} = \vec{c} \odot \vec{1} = \vec{c} \\ \\
    & \Rightarrow M_{N, n} = \vec{m}^{T}U_{N, n}\vec{m} = \vec{c}^{T}U_{N, n}\vec{c} = C_{N, n} 
\end{align*}

\begin{align*}
    & \\ \\
    & f(z) = \sum_{n = 0}^{N - 1}c_{n}z^{-n} \\ \\
    &\Rightarrow |f(\omega)|^{2} = \big|\vec{c}\big|^{2} + 2\sum_{n=1}^{N - 1}C_{N, n}T_{n}\Big(\cos\big(\omega\big)\Big) 
\end{align*}

\end{document}
